src/nextgen_soundness.v
@@ -1,28 +1,103 @@
-From iris.proofmode Require Import classes tactics.
-From iris.base_logic.lib Require Export iprop own invariants fancy_updates wsat later_credits.
+From iris.proofmode Require Import classes tactics proofmode.
+From iris.base_logic.lib Require Export iprop own later_credits.
 From iris.prelude Require Import options.
+From stdpp Require Export coPset.
+
+From iris.algebra Require Import gmap_view gset coPset.
 
 From nextgen Require Import cmra_morphism_extra.
-From nextgen Require Export nextgen_basic.
+From nextgen.lib Require Import wsat fancy_updates.
+From nextgen Require Export nextgen_basic nextgen_pointwise.
 Import uPred.
 
-
-Lemma bnextgen_fupd_soundness_no_lc_alt `{!invGpreS Σ} (E1 : coPset) (P : iProp Σ) `{!Plain P} m (f : iResUR Σ -> iResUR Σ) `{GenTrans (iResUR Σ) f} :
-  (∀ `{Hinv: !invGS_gen HasNoLc Σ} `{ω : coPset → iProp Σ}, £ m ∗ (□ (∀ (E0 E3 : coPset) (P0 : iPropI Σ), (|={E0,E3}=> P0) -∗ ω E0 ==∗ ◇ (ω E3 ∗ P0))) ∗ ω E1 ==∗ ⚡={f}=> P) → ⊢ P.
+Local Lemma lc_alloc `{!lcGIndpreS Σ Ω} n :
+  ⊢ |==> ∃ _ : lcGIndS Σ Ω, later_credits.lc_supply n ∗ £ n.
 Proof.
-  intros Hfupd. apply later_soundness.
-  eapply (bnextgen_plain_soundness f); [by apply later_plain|].
-  apply bupd_soundness;[by apply plain_bnextgen_plain,later_plain|].
-  iMod fupd_soundness_no_lc_unfold as (hws ω) "(Hlc & Hω & #H)".
-  iMod (Hfupd with "[$Hlc $H $Hω]"). iModIntro;iFrame.
-  iApply (bnextgen_mono with "[$]"). iIntros "H". iNext. auto.
+  set (WW:=lcGIndpreS0).
+  destruct lcGIndpreS0.
+  rewrite later_credits.lc_unseal /later_credits.lc_def later_credits.lc_supply_unseal /later_credits.lc_supply_def.
+  iMod (own_alloc (● n ⋅ ◯ n)) as (γLC) "[H● H◯]";
+    first (apply auth_both_valid; split; done).
+  pose (C := LcGIndS _ _ lcGpreS_inG γLC).
+  iModIntro. iExists C. iFrame.
 Qed.
 
-Lemma bnextgen_fupd_soundness_no_lc `{!invGpreS Σ} E1 E2 (P : iProp Σ) `{!Plain P} m (f : iResUR Σ -> iResUR Σ) `{GenTrans (iResUR Σ) f} :
-  (∀ `{Hinv: !invGS_gen HasNoLc Σ}, £ m ={E1,E2}=∗ ⚡={f}=> P) → ⊢ P.
+Local Lemma fupd_soundness_no_lc_unfold_alt `{!invGIndpreS Σ Ω} `{!noTransInG Σ Ω T} m E :
+  ⊢ |==> ∃ `(Hws: invGIndS_gen HasNoLc Σ Ω) (ω : coPset -> iProp Σ),
+      £ m ∗ ω E ∗ ■ (∀ E1 E2 P n, (|={E1}[E2]▷=>^n P) -∗ ω E1 -∗ Nat.iter n (λ P, |==> ▷ |==> ▷ P) (ω E1 ∗ P))
+        ∗ ■ (∀ (E1 E2 : coPset) (P : iPropI Σ), (|={E1,E2}=> P) -∗ ω E1 ==∗ ◇ (ω E2 ∗ P))
+        ∗ ■ (∀ E (t : T → T) `{!CmraMorphism t}, ω E -∗ ⚡={transmap_insert_inG t Ω}=> ω E).
+Proof.
+  destruct invGIndpreS0.
+  iMod wsat_alloc as (Hw) "[Hw HE]".
+  (* We don't actually want any credits, but we need the [lcGS]. *)
+  iMod (lc_alloc m) as (Hc) "[Hsupply Hm]".
+  set (Hi := InvIndG HasNoLc _ Ω Hw Hc).
+  iExists Hi, (λ E, wsat ∗ ownE E)%I.
+  rewrite (union_difference_L E ⊤); [|set_solver].
+  rewrite wsat.ownE_op; [|set_solver]. iFrame.
+  iDestruct "HE" as "[HE _]". iFrame.
+  iModIntro. iSplit;[|iSplit].
+  { iIntros "!>" (E1 E2 P n) "HP HwE".
+    iInduction (n) as [|n] "IH" forall (P).
+    - simpl. iFrame.
+    - assert ((S n) = n + 1) as ->;[lia|].
+      rewrite step_fupdN_add.
+      iDestruct ("IH" with "HP HwE") as "t". simpl.
+      rewrite PeanoNat.Nat.add_1_r.
+      rewrite Nat.iter_succ_r.
+      iApply (iter_modal_mono with "[] t").
+      { intros. iIntros "H H'". iMod "H'". iIntros "!>!>".
+        iMod "H'". iIntros "!>!>". iApply "H". auto. }
+      iIntros "[[Hw HE] HP]".
+      iCombine "Hw HE" as "HwE".
+      rewrite fancy_updates.uPred_fupd_unseal
+        /fancy_updates.uPred_fupd_def -assoc /=.
+      iMod ("HP" with "HwE") as ">[Hwsat [HwE HP]]".
+      iDestruct ("HP" with "[$Hwsat $HwE]") as "Hr".
+      iModIntro. iNext. simpl. iMod "Hr". iModIntro. iMod "Hr". iNext. iFrame. }
+  { iIntros "!>" (E1 E2 P) "HP [Hw HE]".
+    rewrite fancy_updates.uPred_fupd_unseal
+          /fancy_updates.uPred_fupd_def -assoc /=.
+    iMod ("HP" with "[$Hw $HE]") as ">(Hw & HE & HP)". by iFrame. }
+  { iModIntro. iIntros (E1 t ?) "[Hw HE]".
+    iDestruct (wsat_ind_insert_intro with "Hw") as "Hw".
+    iDestruct (ownE_ind_insert_intro with "HE") as "HE".
+    iModIntro. iFrame. }
+Qed.
+
+Local Lemma fupd_soundness_no_lc_unfold `{!invGIndpreS Σ Ω} `{!noTransInG Σ Ω T} m E :
+  ⊢ |==> ∃ `(Hws: invGIndS_gen HasNoLc Σ Ω) (ω : coPset → iProp Σ),
+    £ m ∗ ω E ∗ □ (∀ E1 E2 P, (|={E1, E2}=> P) -∗ ω E1 ==∗ ◇ (ω E2 ∗ P)).
+Proof.
+  iMod fupd_soundness_no_lc_unfold_alt as (Hws ω) "(?&?&?&?&?)".
+  iExists Hws,ω. iModIntro. iFrame. eauto.
+Qed.
+
+Local Lemma lc_soundness `{!lcGIndpreS Σ Ω} m (P : iProp Σ) `{!Plain P} :
+  (∀ {Hc: lcGIndS Σ Ω}, £ m -∗ le_upd.le_upd P) → ⊢ P.
+Proof.
+  set (WW:=lcGIndpreS0).
+  destruct lcGIndpreS0.
+  intros H. apply (laterN_soundness _ (S m)).
+  eapply bupd_soundness; first apply _.
+  iStartProof.
+  iMod (lc_alloc m) as (C) "[H● H◯]".
+  iPoseProof (H C) as "Hc". iSpecialize ("Hc" with "H◯").
+  iPoseProof (le_upd.le_upd_elim_complete m with "H● Hc") as "H".
+  simpl. iMod "H". iModIntro. iNext.
+  clear H. iInduction m as [|m] "IH"; simpl; [done|].
+  iMod "H". iNext. by iApply "IH".
+Qed.
+
+Local Notation "⚡={ f }=> P" := (uPred_bnextgen f P)
+                            (at level 99, f at level 50, P at level 200, format "⚡={ f }=>  P") : bi_scope.
+
+Lemma bnextgen_fupd_soundness_no_lc `{!invGIndpreS Σ Ω} `{!noTransInG Σ Ω T} E1 E2 (P : iProp Σ) `{!Plain P} m (f : iResUR Σ -> iResUR Σ) `{GenTrans (iResUR Σ) f}:
+  (∀ `{Hinv: !invGIndS_gen HasNoLc Σ Ω}, £ m ={E1,E2}=∗ ⚡={f}=> P) → ⊢ P.
 Proof.
   intros Hfupd. apply later_soundness.
-  eapply (bnextgen_plain_soundness f); [by apply later_plain|].
+  eapply (bnextgen_plain_soundness); [by apply later_plain|].
   apply bupd_soundness;[by apply plain_bnextgen_plain,later_plain|].
   iMod fupd_soundness_no_lc_unfold as (hws ω) "(Hlc & Hω & #H)".
   iMod ("H" with "[Hlc] Hω") as "H'".
@@ -31,15 +106,15 @@ Proof.
   iDestruct "H2" as ">H2". iModIntro. iNext. iFrame.
 Qed.
 
-Lemma bnextgen_fupd_soundness_lc `{!invGpreS Σ} n E1 E2 (P : iProp Σ) `{!Plain P} (f : iResUR Σ -> iResUR Σ) `{GenTrans (iResUR Σ) f} :
-  (∀ `{Hinv: !invGS_gen HasLc Σ}, £ n ={E1,E2}=∗ ⚡={f}=> P) → ⊢ P.
+Lemma bnextgen_fupd_soundness_lc `{!invGIndpreS Σ Ω} `{!noTransInG Σ Ω T} n E1 E2 (P : iProp Σ) `{!Plain P} (f : iResUR Σ -> iResUR Σ) `{GenTrans (iResUR Σ) f} :
+  (∀ `{Hinv: !invGIndS_gen HasLc Σ Ω}, £ n ={E1,E2}=∗ ⚡={f}=> P) → ⊢ P.
 Proof.
-  inversion invGpreS0.
-  intros Hfupd. eapply (le_upd.lc_soundness (S n)); first done.
+  destruct invGIndpreS0.
+  intros Hfupd. eapply (lc_soundness (S n)); first done.
   intros Hc. rewrite lc_succ.
   iIntros "[Hone Hn]". rewrite -le_upd.le_upd_trans. iApply le_upd.bupd_le_upd.
   iMod wsat_alloc as (Hw) "[Hw HE]".
-  set (Hi := InvG HasLc _ Hw Hc).
+  set (Hi := InvIndG HasLc _ _ Hw Hc).
   iAssert (|={⊤,E2}=> ⚡={f}=> P)%I with "[Hn]" as "H".
   { iMod (fupd_mask_subseteq E1) as "_"; first done. by iApply (Hfupd Hi). }
   rewrite fancy_updates.uPred_fupd_unseal /fancy_updates.uPred_fupd_def.
@@ -49,17 +124,27 @@ Proof.
   iApply bnextgen_plain. iDestruct "H" as "(_ & _ & $)".
 Qed.
 
-Lemma bnextgen_fupd_soundness_gen `{!invGpreS Σ} n hlc E1 E2 (P : iProp Σ) `{!Plain P} (f : iResUR Σ -> iResUR Σ) `{GenTrans (iResUR Σ) f} :
-  (∀ `{Hinv: !invGS_gen hlc Σ}, £ n ={E1,E2}=∗ ⚡={f}=> P) → ⊢ P.
+Lemma bnextgen_fupd_soundness_gen `{!invGIndpreS Σ Ω} `{!noTransInG Σ Ω T} n hlc E1 E2 (P : iProp Σ) `{!Plain P} (f : iResUR Σ -> iResUR Σ) `{GenTrans (iResUR Σ) f} :
+  (∀ `{Hinv: !invGIndS_gen hlc Σ Ω}, £ n ={E1,E2}=∗ ⚡={f}=> P) → ⊢ P.
 Proof.
-  inversion invGpreS0.
+  inversion invGIndpreS0.
   destruct hlc.
   - by apply bnextgen_fupd_soundness_lc.
   - by apply bnextgen_fupd_soundness_no_lc.
 Qed.
 
-Lemma bnextgen_step_fupdN_soundness_no_lc `{!invGpreS Σ} (P : iProp Σ) `{!Plain P} n m (f : iResUR Σ -> iResUR Σ) `{GenTrans (iResUR Σ) f} :
-  (∀ `{Hinv: !invGS_gen HasNoLc Σ}, £ m ={⊤,∅}=∗ |={∅}▷=>^n ⚡={f}=> P) →
+Local Lemma fupd_soundness_no_lc `{!invGIndpreS Σ Ω} `{!noTransInG Σ Ω T} E1 E2 (P : iProp Σ) `{!Plain P} m :
+  (∀ `{Hinv: !invGIndS_gen HasNoLc Σ Ω}, £ m ={E1,E2}=∗ P) → ⊢ P.
+Proof.
+  intros Hfupd. apply later_soundness, bupd_soundness; [by apply later_plain|].
+  iMod fupd_soundness_no_lc_unfold as (hws ω) "(Hlc & Hω & #H)".
+  iMod ("H" with "[Hlc] Hω") as "H'".
+  { iMod (Hfupd with "Hlc") as "H'". iModIntro. iApply "H'". }
+  iDestruct "H'" as "[>H1 >H2]". by iFrame.
+Qed.
+
+Lemma bnextgen_step_fupdN_soundness_no_lc `{!invGIndpreS Σ Ω} `{!noTransInG Σ Ω T} (P : iProp Σ) `{!Plain P} n m (f : iResUR Σ -> iResUR Σ) `{GenTrans (iResUR Σ) f} :
+  (∀ `{Hinv: !invGIndS_gen HasNoLc Σ Ω}, £ m ={⊤,∅}=∗ |={∅}▷=>^n ⚡={f}=> P) →
   ⊢ P.
 Proof.
   intros Hiter.
@@ -74,8 +159,8 @@ Proof.
   iDestruct (plain with "H") as "H". iFrame.
 Qed.
 
-Lemma bnextgen_step_fupdN_soundness_no_lc' `{!invGpreS Σ} (P : iProp Σ) `{!Plain P} n m (f : iResUR Σ -> iResUR Σ) `{GenTrans (iResUR Σ) f} :
-  (∀ `{Hinv: !invGS_gen HasNoLc Σ}, £ m ={⊤}[∅]▷=∗^n ⚡={f}=> P) →
+Lemma bnextgen_step_fupdN_soundness_no_lc' `{!invGIndpreS Σ Ω} `{!noTransInG Σ Ω T} (P : iProp Σ) `{!Plain P} n m (f : iResUR Σ -> iResUR Σ) `{GenTrans (iResUR Σ) f} :
+  (∀ `{Hinv: !invGIndS_gen HasNoLc Σ Ω}, £ m ={⊤}[∅]▷=∗^n ⚡={f}=> P) →
   ⊢ P.
 Proof.
   intros Hiter. eapply (bnextgen_step_fupdN_soundness_no_lc _ n m)=>Hinv.
@@ -86,11 +171,12 @@ Proof.
   simpl. iMod "H". iIntros "!>!>!>". iMod "H". by iApply "IH".
 Qed.
 
-Lemma bnextgen_step_fupdN_soundness_lc `{!invGpreS Σ} (P : iProp Σ) `{!Plain P} n m (f : iResUR Σ -> iResUR Σ) `{GenTrans (iResUR Σ) f} :
-  (∀ `{Hinv: !invGS_gen HasLc Σ}, £ m ={⊤,∅}=∗ |={∅}▷=>^n ⚡={f}=> P) →
+
+Lemma bnextgen_step_fupdN_soundness_lc `{!invGIndpreS Σ Ω} `{!noTransInG Σ Ω T} (P : iProp Σ) `{!Plain P} n m (f : iResUR Σ -> iResUR Σ) `{GenTrans (iResUR Σ) f} :
+  (∀ `{Hinv: !invGIndS_gen HasLc Σ Ω}, £ m ={⊤,∅}=∗ |={∅}▷=>^n ⚡={f}=> P) →
   ⊢ P.
 Proof.
-  inversion invGpreS0.
+  inversion invGIndpreS0.
   intros Hiter.
   eapply (bnextgen_fupd_soundness_lc (m + n)); [apply _..|].
   iIntros (Hinv) "Hlc". rewrite lc_split.
@@ -99,15 +185,15 @@ Proof.
   iInduction n as [|n] "IH"; simpl.
   - by iModIntro.
   - rewrite lc_succ. iDestruct "Hn" as "[Hone Hn]".
-    iMod "Hupd". iMod (lc_fupd_elim_later with "Hone Hupd") as "> Hupd".
+    iMod "Hupd". iMod (fancy_updates.lc_fupd_elim_later with "Hone Hupd") as "> Hupd".
     by iApply ("IH" with "Hn Hupd").
 Qed.
 
-Lemma bnextgen_step_fupdN_soundness_lc' `{!invGpreS Σ} (P : iProp Σ) `{!Plain P} n m (f : iResUR Σ -> iResUR Σ) `{GenTrans (iResUR Σ) f} :
-  (∀ `{Hinv: !invGS_gen hlc Σ}, £ m ={⊤}[∅]▷=∗^n ⚡={f}=> P) →
+Lemma bnextgen_step_fupdN_soundness_lc' `{!invGIndpreS Σ Ω} `{!noTransInG Σ Ω T} (P : iProp Σ) `{!Plain P} n m (f : iResUR Σ -> iResUR Σ) `{GenTrans (iResUR Σ) f} :
+  (∀ `{Hinv: !invGIndS_gen hlc Σ Ω}, £ m ={⊤}[∅]▷=∗^n ⚡={f}=> P) →
   ⊢ P.
 Proof.
-  inversion invGpreS0.
+  inversion invGIndpreS0.
   intros Hiter.
   eapply (bnextgen_fupd_soundness_lc (m + n) ⊤ ⊤); [apply _..|].
   iIntros (Hinv) "Hlc". rewrite lc_split.
@@ -117,19 +203,19 @@ Proof.
   iInduction n as [|n] "IH"; simpl.
   - by iModIntro.
   - rewrite lc_succ. iDestruct "Hn" as "[Hone Hn]".
-    iMod "Hupd". iMod (lc_fupd_elim_later with "Hone Hupd") as "> Hupd".
+    iMod "Hupd". iMod (fancy_updates.lc_fupd_elim_later with "Hone Hupd") as "> Hupd".
     by iApply ("IH" with "Hn Hupd").
 Qed.
 
 (** Generic soundness lemma for the fancy update, parameterized by [use_credits]
   on whether to use credits or not. *)
-Lemma bnextgen_step_fupdN_soundness_gen `{!invGpreS Σ} (P : iProp Σ) `{!Plain P}
+Lemma bnextgen_step_fupdN_soundness_gen `{!invGIndpreS Σ Ω} `{!noTransInG Σ Ω T} (P : iProp Σ) `{!Plain P}
   (hlc : has_lc) (n m : nat) (f : iResUR Σ -> iResUR Σ) `{GenTrans (iResUR Σ) f} :
-  (∀ `{Hinv : invGS_gen hlc Σ},
+  (∀ `{Hinv : invGIndS_gen hlc Σ Ω},
     £ m ={⊤,∅}=∗ |={∅}▷=>^n ⚡={f}=> P) →
   ⊢ P.
 Proof.
-  inversion invGpreS0.
+  inversion invGIndpreS0.
   destruct hlc.
   - apply bnextgen_step_fupdN_soundness_lc. done.
   - apply bnextgen_step_fupdN_soundness_no_lc. done.
@@ -161,28 +247,41 @@ Proof.
     iMod "H1". iMod "H2".
     iModIntro. iApply IHn. iFrame.
 Qed.
-  
+
+Local Notation "⚡={ M }=> P" := (nextgen_omega M P)
+  (at level 99, M at level 50, P at level 200, format "⚡={ M }=>  P") : bi_scope.
 
 Section bnextgen_pred_imod.
-  Context {M : ucmra} {A : Type} (f : A -> M → M) `{!forall a, CmraMorphism (f a)} {num_laters_per_step : nat -> nat}
-    `{BiFUpd (uPredI M)}.
+  Context {Σ : gFunctors} {Ω : gTransformations Σ} {A : Type} `{!noTransInG Σ Ω C} (f : A -> C → C) `{!forall a, CmraMorphism (f a)} {num_laters_per_step : nat -> nat}
+  `{!invGIndS_gen hlc Σ Ω}.
 
+  
+  Fixpoint bnextgen_repeat_n
+    (l : list A) (P : iProp Σ) : iProp Σ :=
+    match l with
+    | [] => P
+    | a :: l' => ⚡={transmap_insert_inG (f a) Ω}=> (bnextgen_repeat_n l' P)
+    end.
+  
   Fixpoint bnextgen_n
-    (l : list A) (start : nat) (P : uPredI M) : uPredI M :=
+    (l : list A) (start : nat) (P : iProp Σ) : iProp Σ :=
     match l with
     | [] => P
     | a :: l' => |={⊤,∅}=> |={∅}▷=>^(S $ num_laters_per_step start) |={∅,⊤}=>
-        ⚡={f a}=> (bnextgen_n l' (S start) P)
+        ⚡={transmap_insert_inG (f a) Ω}=> (bnextgen_n l' (S start) P)
     end.
   
   Fixpoint bnextgen_n_open
-    (l : list A) (start : nat) (P : uPredI M) : uPredI M :=
+    (l : list A) (start : nat) (P : iProp Σ) : iProp Σ :=
     match l with
     | [] =>  P
     | a :: l' => |={∅}▷=>^(S $ num_laters_per_step start)
-                          ⚡={f a}=> (bnextgen_n_open l' (S start) P)
+                          ⚡={transmap_insert_inG (f a) Ω}=> (bnextgen_n_open l' (S start) P)
     end.
 
+  Notation "⚡={[ l ]}=> P" := (bnextgen_repeat_n l P)
+         (at level 99, l at level 50, P at level 200, format "⚡={[ l ]}=> P") : bi_scope.
+  
   Notation "⚡={[ l ]}▷=>^ ( n ) P" := (bnextgen_n l n P)
          (at level 99, l at level 50, n at level 50, P at level 200, format "⚡={[ l ]}▷=>^ ( n )  P") : bi_scope.
 
@@ -234,7 +333,7 @@ Section bnextgen_pred_imod.
     Proper ((≡) ==> (≡)) (bnextgen_n l n) := ne_proper _.
 
   Lemma bnextgen_n_open_snoc l x n P :
-    (⚡={[(l ++ [x])]}▷=>>^(n) P) ⊣⊢ ⚡={[l]}▷=>>^(n) (|={∅}▷=> |={∅}▷=>^(num_laters_per_step (n + length l)) ⚡={f x}=> P).
+    (⚡={[(l ++ [x])]}▷=>>^(n) P) ⊣⊢ ⚡={[l]}▷=>>^(n) (|={∅}▷=> |={∅}▷=>^(num_laters_per_step (n + length l)) ⚡={transmap_insert_inG (f x) Ω}=> P).
   Proof.
     revert n; induction l => n.
     - simpl. iSplit; iIntros "H"; rewrite Nat.add_0_r; auto.
@@ -248,7 +347,7 @@ Section bnextgen_pred_imod.
   Qed.
 
   Lemma bnextgen_n_snoc l x n P :
-    (⚡={[(l ++ [x])]}▷=>^(n) P) ⊣⊢ ⚡={[l]}▷=>^(n) (|={⊤,∅}=> |={∅}▷=> |={∅}▷=>^(num_laters_per_step (n + length l)) |={∅,⊤}=> ⚡={f x}=> P).
+    (⚡={[(l ++ [x])]}▷=>^(n) P) ⊣⊢ ⚡={[l]}▷=>^(n) (|={⊤,∅}=> |={∅}▷=> |={∅}▷=>^(num_laters_per_step (n + length l)) |={∅,⊤}=> ⚡={transmap_insert_inG (f x) Ω}=> P).
   Proof.
     revert n; induction l => n.
     - simpl. iSplit; iIntros "H"; rewrite Nat.add_0_r; auto. (* rewrite fupd_trans. auto. *)
@@ -275,46 +374,52 @@ Section bnextgen_pred_imod.
       iMod "H1". iModIntro. iModIntro. iApply IHl.
       iFrame.
   Qed.
-  
-End bnextgen_pred_imod.
 
-Lemma fupd_soundness_no_lc_unfold_alt `{!invGpreS Σ} m E :
-  ⊢ |==> ∃ `(Hws: invGS_gen HasNoLc Σ) (ω : coPset → iProp Σ),
-      £ m ∗ ω E ∗ ■ (∀ E1 E2 P n, (|={E1}[E2]▷=>^n P) -∗ ω E1 -∗ Nat.iter n (λ P, |==> ▷ |==> ▷ P) (ω E1 ∗ P))
-                ∗ ■ (∀ (E1 E2 : coPset) (P : iPropI Σ), (|={E1,E2}=> P) -∗ ω E1 ==∗ ◇ (ω E2 ∗ P)).
-Proof.
-  inversion invGpreS0.
-  iMod wsat_alloc as (Hw) "[Hw HE]".
-  (* We don't actually want any credits, but we need the [lcGS]. *)
-  iMod (later_credits.le_upd.lc_alloc m) as (Hc) "[_ Hlc]".
-  set (Hi := InvG HasNoLc _ Hw Hc).
-  iExists Hi, (λ E, wsat ∗ ownE E)%I.
-  rewrite (union_difference_L E ⊤); [|set_solver].
-  rewrite ownE_op; [|set_solver].
-  iDestruct "HE" as "[HE _]". iFrame.
-  iModIntro. iSplit.
-  { iIntros "!>" (E1 E2 P n) "HP HwE".
-    iInduction (n) as [|n] "IH" forall (P).
-    - simpl. iFrame.
-    - assert ((S n) = n + 1) as ->;[lia|].
-      rewrite step_fupdN_add.
-      iDestruct ("IH" with "HP HwE") as "t". simpl.
-      rewrite PeanoNat.Nat.add_1_r.
-      rewrite Nat.iter_succ_r.
-      iApply (iter_modal_mono with "[] t").
-      { intros. iIntros "H H'". iMod "H'". iIntros "!>!>".
-        iMod "H'". iIntros "!>!>". iApply "H". auto. }
-      iIntros "[HwE HP]".
-      rewrite fancy_updates.uPred_fupd_unseal
-        /fancy_updates.uPred_fupd_def -assoc /=.
-      iMod ("HP" with "HwE") as ">[Hwsat [HwE HP]]".
-      iDestruct ("HP" with "[$Hwsat $HwE]") as "Hr".
-      iModIntro. iNext. iMod "Hr". iModIntro. iMod "Hr". iNext. auto. }
-  { iIntros "!>" (E1 E2 P) "HP HwE".
-    rewrite fancy_updates.uPred_fupd_unseal
-          /fancy_updates.uPred_fupd_def -assoc /=.
-    by iApply ("HP" with "HwE"). }
-Qed.
+  Lemma bnextgen_n_sep_nextgen l n P Q :
+    (⚡={[ l ]}=> P) ∗ (⚡={[ l ]}▷=>^(n) Q) -∗ ⚡={[ l ]}▷=>^(n) P ∗ Q.
+  Proof.
+    revert n; induction l =>n.
+    - simpl. iIntros "H". auto.
+    - simpl. iIntros "[H1 H2]".
+      iMod "H2". iModIntro.
+      iApply (step_fupdN_wand with "H2").
+      iNext. iIntros "H2".
+      iMod "H2". iModIntro. iModIntro. iApply IHl.
+      iFrame.
+  Qed.
+
+  Lemma bnextgen_n_open_emp_intro P l n :
+    (⊢ P) -> ⊢ (⚡={[ l ]}▷=>>^(n) P).
+  Proof.
+    intros HP.
+    revert n; induction l =>n;simpl;auto.
+    iApply step_fupdN_intro;auto.
+    iModIntro. iNext. iModIntro.
+    iNext. iModIntro. iStopProof;eauto.
+    apply IHl.
+  Qed.
+
+  Lemma bnextgen_n_emp_intro P l n :
+    (⊢ P) -> ⊢ (⚡={[ l ]}▷=>^(n) P).
+  Proof.
+    intros HP.
+    revert n; induction l =>n;simpl;auto.
+    iApply step_fupdN_intro;auto.
+    iApply fupd_mask_intro;auto. iIntros "Hcls".
+    iModIntro. iNext. iModIntro.
+    iNext. iMod "Hcls". iModIntro. iModIntro. iStopProof;eauto.
+    apply IHl.
+  Qed.
+
+  Lemma bnextgen_repeat_n_emp_intro P l :
+    (⊢ P) -> ⊢ (⚡={[ l ]}=> P).
+  Proof.
+    intros HP.
+    induction l;simpl;auto.
+    iModIntro. auto.
+  Qed.
+    
+End bnextgen_pred_imod.
 
 Lemma bupd_laterN_plain_interweave :
   ∀ {PROP : bi} {BiBUpd0 : BiBUpd PROP} {BiPlainly0 : BiPlainly PROP},
@@ -336,18 +441,18 @@ Fixpoint steps_sum (num_laters_per_step : nat → nat) (start ns : nat) : nat :=
   end.
 
 Section bnextgen_n_open_soundness.
-  Context {A : Type} {Σ : gFunctors} (f : A -> iResUR Σ → iResUR Σ) `{!forall a, CmraMorphism (f a)}
+  Context {A : Type} {Σ : gFunctors} {Ω : gTransformations Σ} `{!noTransInG Σ Ω C} (f : A -> C → C) `{!forall (a : A), CmraMorphism (f a)}
     {num_laters_per_step : nat -> nat}.
 
-  Notation "⚡={[ l ]}▷=>^ ( n ) P" := (@bnextgen_n _ _ f _ num_laters_per_step _ l n P)
+  Notation "⚡={[ l ]}▷=>^ ( n ) P" := (@bnextgen_n _ _ _ _ _ f _ num_laters_per_step _ _ l n P)
          (at level 99, l at level 50, n at level 50, P at level 200, format "⚡={[ l ]}▷=>^ ( n )  P") : bi_scope.
 
-  Notation "⚡={[ l ]}▷=>>^ ( n ) P" := (@bnextgen_n_open _ _ f _ num_laters_per_step _ l n P)
+  Notation "⚡={[ l ]}▷=>>^ ( n ) P" := (@bnextgen_n_open _ _ _ _ _ f _ num_laters_per_step _ _ l n P)
          (at level 99, l at level 50, n at level 50, P at level 200, format "⚡={[ l ]}▷=>>^ ( n )  P") : bi_scope.
 
   Lemma step_fupdN_nextgen_open_soundness_no_lc (l : list A) :
-    invGpreS Σ → ∀ P : iProp Σ,
-        Plain P → ∀ (n m : nat), (∀ (Hinv : invGS_gen HasNoLc Σ), £ m -∗ ⚡={[l]}▷=>>^(n) (* |={⊤,∅}=> *) P) → (⊢ P)%stdpp.
+    invGIndpreS Σ Ω → ∀ P : iProp Σ,
+        Plain P → ∀ (n m : nat), (∀ (Hinv : invGIndS_gen HasNoLc Σ Ω), £ m -∗ ⚡={[l]}▷=>>^(n) P) → (⊢ P)%stdpp.
   Proof.
     intros until P. intros HPlain n m  Hiter.
     apply (laterN_soundness _ (steps_sum num_laters_per_step (n) (S (length l)) + steps_sum num_laters_per_step (n) (S (length l)))).
@@ -355,11 +460,11 @@ Section bnextgen_n_open_soundness.
     specialize (Hiter Hws).
     rewrite lc_split. iDestruct "Hm" as "[Hm Hn]".
     iDestruct (Hiter with "Hm") as "HH". clear Hiter.
-    iStopProof. revert n. induction l;intros n;iIntros "[#[H H'] (Hn & Hω & HH)]".
+    iStopProof. revert n. induction l;intros n;iIntros "[#[H [H' Hintro]] (Hn & Hω & HH)]".
     - simpl. auto.
     - simpl. rewrite /= -Nat.add_succ_r.
       iDestruct "Hn" as "[Hone [Hm Hn]]".
-      iAssert (|={∅}▷=>^(S $ num_laters_per_step n) ⚡={f a}=> ⚡={[l]}▷=>>^(S n) P)%I with "HH" as "HH".
+      iAssert (|={∅}▷=>^(S $ num_laters_per_step n) ⚡={transmap_insert_inG (f a) Ω}=> ⚡={[l]}▷=>>^(S n) P)%I with "HH" as "HH".
       iDestruct ("H" with "HH Hω") as "HH".
 
       set (num:=S (num_laters_per_step (S n) + steps_sum num_laters_per_step (S (S n)) (length l))).
@@ -373,18 +478,19 @@ Section bnextgen_n_open_soundness.
       { intros. iIntros "J H". iMod "H". iIntros "!>!>".
         iMod "H". iIntros "!>!>". iApply "J". iFrame. }
       iIntros "[Hω HP]".
-      iApply (bnextgen_plain (f a)).
-      iAssert (⚡={f a}=> ω ∅)%I with "[Hω]" as "HA1";[admit|].
-      iAssert (⚡={f a}=> £ (steps_sum num_laters_per_step (S n) (length l)))%I with "[Hn]" as "HA2";[admit|].
+      iApply (transmap_plain (transmap_insert_inG (f a) Ω)).
+      iAssert (⚡={transmap_insert_inG (f a) Ω}=> ω ∅)%I with "[Hω]" as "HA1".
+      { iApply "Hintro". iFrame. }
+      iDestruct (lc_ind_insert_intro with "Hn") as "HA2".
       iModIntro.
-      iDestruct (IHl with "[$H $H' $HA1 $HA2 $HP]") as "HH".
+      iDestruct (IHl with "[$H $H' $HA1 $HA2 $HP $Hintro]") as "HH".
       rewrite /num. simpl. iNext. iApply (laterN_mono with "HH"). auto.
-  Admitted.
+  Qed.
 
 
   Lemma step_fupdN_nextgen_soundness_no_lc (l : list A) :
-    invGpreS Σ → ∀ P : iProp Σ,
-        Plain P → ∀ (n m : nat), (∀ (Hinv : invGS_gen HasNoLc Σ), £ m ={⊤}=∗ ⚡={[l]}▷=>^(n) |={⊤,∅}=> P) → (⊢ P)%stdpp.
+    invGIndpreS Σ Ω → ∀ P : iProp Σ,
+        Plain P → ∀ (n m : nat), (∀ (Hinv : invGIndS_gen HasNoLc Σ Ω), £ m ={⊤}=∗ ⚡={[l]}▷=>^(n) |={⊤,∅}=> P) → (⊢ P)%stdpp.
   Proof.
     intros until P. inversion H0. intros HPlain n m  Hiter.
     apply (laterN_soundness _ (steps_sum num_laters_per_step (n) (S (length l)) + steps_sum num_laters_per_step (n) (S (length l)))).
@@ -392,18 +498,18 @@ Section bnextgen_n_open_soundness.
     specialize (Hiter Hws).
     rewrite lc_split. iDestruct "Hm" as "[Hm Hn]".
     iDestruct (Hiter with "Hm") as "HH". clear Hiter.
-    iStopProof. revert n. induction l;intros n;iIntros "[#[H H'] (Hn & Hω & HH)]".
+    iStopProof. revert n. induction l;intros n;iIntros "[#[H [H' Hintro]] (Hn & Hω & HH)]".
     - simpl. rewrite fupd_trans.
       iMod ("H'" with "HH Hω") as "[>Hω >HH]". auto.
     - simpl. rewrite /= -Nat.add_succ_r.
       iDestruct "Hn" as "[Hone [Hm Hn]]".
-      rewrite fupd_trans.
+      rewrite (fupd_trans ⊤ ⊤).
 
       iApply bupd_plain.
       iMod ("H'" with "HH Hω") as "[>Hω >HH]".
       iModIntro.
       
-      iAssert (|={∅}▷=>^(S $ num_laters_per_step n) |={∅,⊤}=> ⚡={f a}=> ⚡={[l]}▷=>^(S n) |={⊤,∅}=> P)%I with "HH" as "HH".
+      iAssert (|={∅}▷=>^(S $ num_laters_per_step n) |={∅,⊤}=> ⚡={transmap_insert_inG (f a) Ω}=> ⚡={[l]}▷=>^(S n) |={⊤,∅}=> P)%I with "HH" as "HH".
       iDestruct ("H" with "HH Hω") as "HH".
 
       set (num:=S (num_laters_per_step (S n) + steps_sum num_laters_per_step (S (S n)) (length l))).
@@ -420,14 +526,15 @@ Section bnextgen_n_open_soundness.
 
       iApply bupd_plain.
       iMod ("H'" with "HP Hω") as "[>Hω >HP]".
-      iModIntro.      
-      
-      iApply (bnextgen_plain (f a)).
-      iAssert (⚡={f a}=> ω ⊤)%I with "[Hω]" as "HA1";[admit|].
-      iAssert (⚡={f a}=> £ (steps_sum num_laters_per_step (S n) (length l)))%I with "[Hn]" as "HA2";[admit|].
       iModIntro.
-      iDestruct (IHl with "[$H $H' $HA1 $HA2 $HP]") as "HH";auto.
-  Admitted.
+
+      iApply (transmap_plain (transmap_insert_inG (f a) Ω)).
+      iAssert (⚡={transmap_insert_inG (f a) Ω}=> ω ⊤)%I with "[Hω]" as "HA1".
+      { iApply "Hintro". iFrame. }
+      iDestruct (lc_ind_insert_intro with "Hn") as "HA2".
+      iModIntro.
+      iDestruct (IHl with "[$H $H' $HA1 $HA2 $HP $Hintro]") as "HH";auto.
+  Qed.
   
 
 End bnextgen_n_open_soundness.
