src/lib/fancy_updates.v
@@ -1,0 +1,140 @@
+From stdpp Require Export coPset.
+From iris.algebra Require Import gmap auth agree gset coPset.
+From iris.proofmode Require Import proofmode.
+From iris.base_logic.lib Require Export own.
+From iris.base_logic.lib Require Import wsat.
+From nextgen.lib Require Import wsat.
+From iris.base_logic Require Export later_credits.
+From iris.prelude Require Import options.
+Export wsatGS.
+Import uPred.
+Import le_upd_if.
+From nextgen Require Import nextgen_pointwise.
+
+(** The definition of fancy updates (and in turn the logic built on top of it) is parameterized
+    by whether it supports elimination of laters via later credits or not.
+    This choice is necessary as the fancy update *with* later credits does *not* support
+    the interaction laws with the plainly modality in [BiFUpdPlainly]. While these laws are
+    seldomly used, support for them is required for backwards compatibility.
+
+    Thus, the [invGS_gen] typeclass ("gen" for "generalized") is parameterized by
+    a parameter of type [has_lc] that determines whether later credits are
+    available or not. [invGS] is provided as a convenient notation for the default [HasLc].
+    We don't use that notation in this file to avoid confusion.
+ *)
+
+Class invGIndpreS (Σ : gFunctors) (Ω : gTransformations Σ) : Set := InvGIndpreS {
+  invGIndpreS_wsat : wsatGIndpreS Σ Ω;
+  invGIndpreS_lc : lcGIndpreS Σ Ω;
+}.
+
+Class invGIndS_gen (hlc : fancy_updates.has_lc) (Σ : gFunctors) (Ω : gTransformations Σ) : Set := InvIndG {
+  invGS_wsat : wsatGIndS Σ Ω;
+  invGS_lc : lcGIndS Σ Ω;
+}.
+Global Hint Mode invGIndS_gen - - - : typeclass_instances.
+Global Hint Mode invGIndpreS - - : typeclass_instances.
+
+Local Existing Instances invGIndpreS_wsat invGIndpreS_lc.
+(* [invGS_lc] needs to be global in order to enable the use of lemmas like [lc_split]
+   that require [lcGS], and not [invGS].
+   [invGS_wsat] also needs to be global as the lemmas in [invariants.v] require it. *)
+Global Existing Instances invGS_lc invGS_wsat.
+
+#[global] Instance into_invpres `{Hinv: invGIndpreS Σ Ω} : fancy_updates.invGpreS Σ :=
+  fancy_updates.InvGpreS Σ (@into_wsatpres Σ Ω invGIndpreS_wsat) (@into_lcpres Σ Ω invGIndpreS_lc).
+
+#[global] Instance into_invs `{Hinv: invGIndS_gen hlc Σ Ω} : fancy_updates.invGS_gen hlc Σ :=
+  fancy_updates.InvG hlc Σ (@into_wsats Σ Ω invGS_wsat) (@into_lcs Σ Ω invGS_lc).
+
+Notation has_lc := fancy_updates.has_lc.
+Notation HasLc := fancy_updates.HasLc.
+Notation HasNoLc := fancy_updates.HasNoLc.
+Notation ownE := wsat.ownE.
+Notation ownD := wsat.ownD.
+
+Notation invGIndS := (invGIndS_gen HasLc).
+
+Local Definition uPred_fupd_def `{!invGIndS_gen hlc Σ Ω} `{!noTransInG Σ Ω T} (E1 E2 : coPset) (P : iProp Σ) : iProp Σ :=
+  wsat ∗ ownE E1 -∗ le_upd_if (if hlc is fancy_updates.HasLc then true else false) (◇ (wsat ∗ ownE E2 ∗ P)).
+Local Definition uPred_fupd_aux : seal (@uPred_fupd_def). Proof. by eexists. Qed.
+Definition uPred_fupd := uPred_fupd_aux.(unseal).
+Global Arguments uPred_fupd {hlc Σ _ _ _ _}.
+Local Lemma uPred_fupd_unseal `{!invGIndS_gen hlc Σ Ω} `{!noTransInG Σ Ω T} : @fupd _ uPred_fupd = uPred_fupd_def.
+Proof. rewrite -uPred_fupd_aux.(seal_eq) //. Qed.
+
+Lemma uPred_fupd_mixin `{!invGIndS_gen hlc Σ Ω} `{!noTransInG Σ Ω T} : BiFUpdMixin (uPredI (iResUR Σ)) uPred_fupd.
+Proof.
+  split.
+  - rewrite uPred_fupd_unseal. solve_proper.
+  - intros E1 E2 (E1''&->&?)%subseteq_disjoint_union_L.
+    rewrite uPred_fupd_unseal /uPred_fupd_def ownE_op //.
+    by iIntros "($ & $ & HE) !> !> [$ $] !> !>".
+  - rewrite uPred_fupd_unseal.
+    iIntros (E1 E2 P) ">H [Hw HE]". iApply "H"; by iFrame.
+  - rewrite uPred_fupd_unseal.
+    iIntros (E1 E2 P Q HPQ) "HP HwE". rewrite -HPQ. by iApply "HP".
+  - rewrite uPred_fupd_unseal. iIntros (E1 E2 E3 P) "HP HwE".
+    iMod ("HP" with "HwE") as ">(Hw & HE & HP)". iApply "HP"; by iFrame.
+  - intros E1 E2 Ef P HE1Ef. rewrite uPred_fupd_unseal /uPred_fupd_def ownE_op //.
+    iIntros "Hvs (Hw & HE1 &HEf)".
+    iMod ("Hvs" with "[Hw HE1]") as ">($ & HE2 & HP)"; first by iFrame.
+    iDestruct (ownE_op' with "[HE2 HEf]") as "[? $]"; first by iFrame.
+    iIntros "!> !>". by iApply "HP".
+  - rewrite uPred_fupd_unseal /uPred_fupd_def. by iIntros (????) "[HwP $]".
+Qed.
+Global Instance uPred_bi_fupd `{!invGIndS_gen hlc Σ Ω} `{!noTransInG Σ Ω T} : BiFUpd (uPredI (iResUR Σ)) | 1 :=
+  {| bi_fupd_mixin := uPred_fupd_mixin |}.
+
+Global Instance uPred_bi_bupd_fupd {Σ : gFunctors} `{!invGIndS_gen hlc Σ Ω} `{!noTransInG Σ Ω T} : BiBUpdFUpd (uPredI (iResUR Σ)) | 1.
+Proof. rewrite /BiBUpdFUpd. rewrite uPred_fupd_unseal. by iIntros (E P) ">? [$ $] !> !>". Qed.
+
+(** The interaction laws with the plainly modality are only supported when
+  we opt out of the support for later credits. *)
+Global Instance uPred_bi_fupd_plainly_no_lc `{!invGIndS_gen fancy_updates.HasNoLc Σ Ω} `{!noTransInG Σ Ω T} :
+  BiFUpdPlainly (uPredI (iResUR Σ)) | 1.
+Proof.
+  split; rewrite uPred_fupd_unseal /uPred_fupd_def.
+  - iIntros (E P) "H [Hw HE]".
+    iAssert (◇ ■ P)%I as "#>HP".
+    { by iMod ("H" with "[$]") as "(_ & _ & HP)". }
+    by iFrame.
+  - iIntros (E P Q) "[H HQ] [Hw HE]".
+    iAssert (◇ ■ P)%I as "#>HP".
+    { by iMod ("H" with "HQ [$]") as "(_ & _ & HP)". }
+    by iFrame.
+  - iIntros (E P) "H [Hw HE]".
+    iAssert (▷ ◇ ■ P)%I as "#HP".
+    { iNext. by iMod ("H" with "[$]") as "(_ & _ & HP)". }
+    iFrame. iIntros "!> !> !>". by iMod "HP".
+  - iIntros (E A Φ) "HΦ [Hw HE]".
+    iAssert (◇ ■ ∀ x : A, Φ x)%I as "#>HP".
+    { iIntros (x). by iMod ("HΦ" with "[$Hw $HE]") as "(_&_&?)". }
+    by iFrame.
+Qed.
+
+(** Later credits: the laws are only available when we opt into later credit support.*)
+
+(** [lc_fupd_elim_later] allows to eliminate a later from a hypothesis at an update.
+  This is typically used as [iMod (lc_fupd_elim_later with "Hcredit HP") as "HP".],
+  where ["Hcredit"] is a credit available in the context and ["HP"] is the
+  assumption from which a later should be stripped. *)
+Lemma lc_fupd_elim_later `{!invGIndS_gen HasLc Σ Ω} `{!noTransInG Σ Ω T} E P :
+   £ 1 -∗ (▷ P) -∗ |={E}=> P.
+Proof.
+  iIntros "Hf Hupd".
+  rewrite uPred_fupd_unseal /uPred_fupd_def.
+  iIntros "[$ $]". iApply (le_upd_later with "Hf").
+  iNext. by iModIntro.
+Qed.
+
+(** If the goal is a fancy update, this lemma can be used to make a later appear
+  in front of it in exchange for a later credit.
+  This is typically used as [iApply (lc_fupd_add_later with "Hcredit")],
+  where ["Hcredit"] is a credit available in the context. *)
+Lemma lc_fupd_add_later `{!invGIndS_gen HasLc Σ Ω} `{!noTransInG Σ Ω T} E1 E2 P :
+  £ 1 -∗ (▷ |={E1, E2}=> P) -∗ |={E1, E2}=> P.
+Proof.
+  iIntros "Hf Hupd". iApply (fupd_trans E1 E1).
+  iApply (lc_fupd_elim_later with "Hf Hupd").
+Qed.
