src/utils.v
@@ -2,6 +2,8 @@ From iris.algebra Require Import functions gmap agree excl csum.
 From iris.proofmode Require Import classes tactics.
 From iris.base_logic.lib Require Export iprop own invariants.
 From iris.prelude Require Import options.
+From iris.bi Require Import plainly.
+From iris.bi Require Import derived_laws_later.
 
 Import EqNotations. (* Get the [rew] notation. *)
 
@@ -74,3 +76,23 @@ Section cmra_map_transport.
 
 End cmra_map_transport.
 
+Lemma löb_wand_plainly {M} (P : uPredI M) `{!Absorbing P} :
+    ■ ((■ ▷ P) -∗ P) ⊢ P.
+Proof.
+  rewrite -{3}(plainly_elim P) -(bi.löb (■ P)%I).
+  apply bi.impl_intro_l. rewrite later_plainly_1.
+  rewrite -{1}(plainly_idemp (▷ P)).
+  rewrite -plainly_and plainly_and_sep. rewrite bi.wand_elim_r. auto.
+Qed.
+
+Lemma löb_wand_plainly_and_intuitionistically {M} (P : uPredI M) `{!Absorbing P} :
+  □ ■ ((□ ■ ▷ P) -∗ P) ⊢ P.
+Proof.
+  rewrite -{3}(plainly_elim P) -{1}(bi.intuitionistically_elim (■ P)%I) -(bi.löb (□ ■ P)%I).
+  apply bi.impl_intro_l. rewrite bi.later_intuitionistically later_plainly_1.
+  rewrite -{1}(plainly_idemp (▷ P)).
+  rewrite -{1}(bi.intuitionistically_idemp (■ ■ ▷ P)%I).
+  rewrite intuitionistically_plainly.
+  rewrite bi.and_sep_intuitionistically.
+  rewrite bi.intuitionistically_sep_2 -plainly_sep. rewrite bi.wand_elim_r. auto.
+Qed.
